Superposition_Calculus/First_Order_Superposition_Completeness.thy
@@ -22,7 +22,7 @@ hide_const
 context grounded_first_order_superposition_calculus
 begin
 
-
+ (* TODO: term "Nonground_Clause.clause.subst"*)
 lemma eq_resolution_lifting:
   fixes 
     premise\<^sub>G conclusion\<^sub>G :: "'f gatom clause" and 
@@ -88,15 +88,15 @@ proof(cases premise\<^sub>G conclusion\<^sub>G rule: ground.ground_eq_resolution
   moreover have max_literal_\<gamma>: "max_literal \<cdot>l \<gamma> = literal.from_ground (term\<^sub>G !\<approx> term\<^sub>G)"
     if ?select\<^sub>G_empty
   proof-
-    have "literal.order.restriction.is_maximal literal\<^sub>G premise\<^sub>G"
+    have "ground_is_maximal literal\<^sub>G premise\<^sub>G"
       using ground_eq_resolutionI(3) that maximal_in_clause
-      by (metis literal.order.restriction.is_maximal_empty)
+      unfolding is_maximal_def
+      by (simp add: clause_from_ground_empty_mset)
 
     then show ?thesis
       using max_literal(2) unique_maximal_in_ground_clause[OF premise_grounding] 
       unfolding 
         ground_eq_resolutionI(2) 
-        ground_is_maximal_iff_is_maximal
         premise\<^sub>G 
         clause.to_ground_inverse[OF premise_grounding]
       by blast
@@ -107,7 +107,7 @@ proof(cases premise\<^sub>G conclusion\<^sub>G rule: ground.ground_eq_resolution
     "is_maximal selected_literal (select premise)" 
   if ?select\<^sub>G_not_empty
   proof-
-    have "literal.order.restriction.is_maximal literal\<^sub>G (select\<^sub>G premise\<^sub>G)" if ?select\<^sub>G_not_empty
+    have "ground_is_maximal literal\<^sub>G (select\<^sub>G premise\<^sub>G)" if ?select\<^sub>G_not_empty
       using ground_eq_resolutionI(3) that
       by blast
 
@@ -120,7 +120,6 @@ proof(cases premise\<^sub>G conclusion\<^sub>G rule: ground.ground_eq_resolution
       unfolding
         ground_eq_resolutionI(2) 
         premise\<^sub>G
-        ground_is_maximal_iff_is_maximal
       by (metis (full_types) clause_subst_empty(2) clause.from_ground_inverse clause_to_ground_empty_mset) 
   qed
 
@@ -223,7 +222,7 @@ proof(cases premise\<^sub>G conclusion\<^sub>G rule: ground.ground_eq_resolution
 
       have "is_maximal (literal \<cdot>l \<gamma>) (select premise \<cdot> \<gamma>)"
         using False ground_eq_resolutionI(3) 
-        unfolding ground_eq_resolutionI(2) ground_is_maximal_iff_is_maximal literal_\<gamma> select
+        unfolding ground_eq_resolutionI(2) literal_\<gamma> select
         by presburger
 
       then have "is_maximal (literal \<cdot>l \<mu>) (select premise \<cdot> \<mu>)"
@@ -329,7 +328,6 @@ proof(cases premise\<^sub>G conclusion\<^sub>G rule: ground.ground_eq_factoring.
   have max_ground_literal: "is_maximal (literal.from_ground (term\<^sub>G\<^sub>1 \<approx> term\<^sub>G\<^sub>2)) (premise \<cdot> \<gamma>)"
     using ground_eq_factoringI(5)
     unfolding 
-      ground_is_maximal_iff_is_maximal
       ground_eq_factoringI(2) 
       premise\<^sub>G 
       clause.to_ground_inverse[OF premise_grounding].
@@ -638,7 +636,6 @@ proof(cases premise\<^sub>G\<^sub>2 premise\<^sub>G\<^sub>1 conclusion\<^sub>G r
   have pos_literal\<^sub>G\<^sub>1_is_strictly_maximal\<^sub>l: 
     "is_strictly_maximal (literal.from_ground literal\<^sub>G\<^sub>1) (premise\<^sub>1 \<cdot> \<rho>\<^sub>1 \<odot> \<gamma>)" if "\<P>\<^sub>G = Pos"
     using ground_superpositionI(9) that
-    unfolding ground_is_strictly_maximal_iff_is_strictly_maximal
     by(simp add: premise\<^sub>1_grounding)
 
   have neg_literal\<^sub>G\<^sub>1_is_maximal\<^sub>l: 
@@ -649,9 +646,7 @@ proof(cases premise\<^sub>G\<^sub>2 premise\<^sub>G\<^sub>1 conclusion\<^sub>G r
       is_maximal_if_is_strictly_maximal 
       is_maximal_empty
       premise\<^sub>1_\<gamma>
-    unfolding 
-      ground_is_maximal_iff_is_maximal
-      ground_is_strictly_maximal_iff_is_strictly_maximal
+    unfolding
       ground_superpositionI(1)
    (* TODO: *)
     apply auto
@@ -690,7 +685,7 @@ proof(cases premise\<^sub>G\<^sub>2 premise\<^sub>G\<^sub>1 conclusion\<^sub>G r
     "neg_selected_literal\<^sub>1 \<cdot>l \<rho>\<^sub>1 \<odot> \<gamma> = literal.from_ground literal\<^sub>G\<^sub>1" 
   if "\<P>\<^sub>G = Neg" ?select\<^sub>G_not_empty 
   proof-
-    have "literal.order.restriction.is_maximal literal\<^sub>G\<^sub>1 (select\<^sub>G premise\<^sub>G\<^sub>1)" if "\<P>\<^sub>G = Neg" ?select\<^sub>G_not_empty
+    have "ground_is_maximal literal\<^sub>G\<^sub>1 (select\<^sub>G premise\<^sub>G\<^sub>1)" if "\<P>\<^sub>G = Neg" ?select\<^sub>G_not_empty
       using ground_superpositionI(9) that
       by simp
 
@@ -700,7 +695,7 @@ proof(cases premise\<^sub>G\<^sub>2 premise\<^sub>G\<^sub>1 conclusion\<^sub>G r
         select(1) 
         unique_maximal_in_ground_clause
         obtain_maximal_literal
-      unfolding premise\<^sub>G\<^sub>1 ground_is_maximal_iff_is_maximal
+      unfolding premise\<^sub>G\<^sub>1
       by (metis (mono_tags, lifting) clause.comp_subst.monoid_action_compatibility 
           clause_subst_empty(2) clause.ground_is_ground image_mset_is_empty_iff 
           clause.from_ground_def)
@@ -724,7 +719,6 @@ proof(cases premise\<^sub>G\<^sub>2 premise\<^sub>G\<^sub>1 conclusion\<^sub>G r
   have literal\<^sub>G\<^sub>2_is_strictly_maximal\<^sub>l: 
     "is_strictly_maximal (literal.from_ground literal\<^sub>G\<^sub>2) (premise\<^sub>2 \<cdot> \<rho>\<^sub>2 \<odot> \<gamma>)"
     using ground_superpositionI(11)
-    unfolding ground_is_strictly_maximal_iff_is_strictly_maximal
     by (simp add: premise\<^sub>2_grounding)
 
   obtain literal\<^sub>2 where 
@@ -1516,7 +1510,7 @@ proof(cases premise\<^sub>G\<^sub>2 premise\<^sub>G\<^sub>1 conclusion\<^sub>G r
 
           have "is_maximal (literal\<^sub>1  \<cdot>l \<rho>\<^sub>1 \<cdot>l \<gamma>) (select premise\<^sub>1 \<cdot> \<rho>\<^sub>1 \<cdot> \<gamma>)"  
             using select\<^sub>G_not_empty ground_superpositionI(9) \<P>\<^sub>G_Neg 
-            unfolding ground_is_maximal_iff_is_maximal literal\<^sub>1_\<gamma>[symmetric] select(1)
+            unfolding literal\<^sub>1_\<gamma>[symmetric] select(1)
             by simp
 
           then have "is_maximal (literal\<^sub>1 \<cdot>l \<rho>\<^sub>1 \<cdot>l \<mu>) ((select premise\<^sub>1) \<cdot> \<rho>\<^sub>1 \<cdot> \<mu>)"
